tape_contains v3 MatchNat

TM/Code/MatchNat.v
@@ -9,6 +9,8 @@ Lemma encode_nat_correct (n : nat) :
   encode n = repeat true n ++ [false].
 Proof. induction n; cbn in *; f_equal; auto. Qed.
 
+Local Arguments Encode_Nat : simpl never.
+
 
 
 (* Basic pattern matching *)
@@ -27,107 +29,49 @@ Section MatchNat.
            end).
 
   Definition MatchNat : { M : mTM (bool^+) 1 & states M -> bool } :=
+    Move _ R tt;;
     MATCH (Read_char _)
           (fun o => match o with
-                 | Some (inr true)  => Write (inl START) tt;; Move _ R true  (* S *)
-                 | Some (inr false) => mono_Nop _ false (* O *)
+                 | Some (inr true)  => Write (inl START) true (* S *)
+                 | Some (inr false) => Move _ L false (* O *)
                  | _ => mono_Nop _ true (* invalid input *)
                  end).
 
   Lemma MatchNat_Sem : MatchNat ⊨c(5) MatchNat_Rel.
   Proof.
     eapply RealiseIn_monotone.
-    {
-      unfold MatchNat. eapply Match_RealiseIn. cbn. eapply read_char_sem.
-      instantiate (2 := fun o : option (bool^+) =>
-                          match o with Some (inr true) => _ | Some (inr false) => _ | _ => _ end).
-      cbn. intros [ s | ]; cbn.
-      - destruct s as [ start | s]; cbn.
-        + eapply RealiseIn_monotone'. eapply mono_Nop_Sem. omega.
-        + destruct s.
-          * eapply Seq_RealiseIn; [eapply Write_Sem | eapply Move_Sem].
-          * eapply mono_Nop_Sem.
-      - eapply RealiseIn_monotone'. eapply mono_Nop_Sem. omega.
-    }
-    { cbn. omega. }
+    { unfold MatchNat. repeat TM_Correct. }
+    { Unshelve. 4,6: reflexivity. all: omega. }
     {
       intros tin (yout&tout) H. intros n HEncN. TMSimp.
-      destruct HEncN as (x&ys&r1&HE1&HE2).
-      rewrite encode_nat_correct in HE1.
-      rewrite HE2 in H0. cbn in *.
-      destruct n; cbn in *; inv HE1; TMSimp; cbn.
+      destruct HEncN as (r1&HEncN). rewrite encode_nat_correct in HEncN. TMSimp.
+      destruct n; cbn in *; TMSimp.
       - repeat econstructor.
-      - destruct n; cbn.
-        + repeat econstructor.
-        + split; auto. hnf. do 3 eexists. split. rewrite encode_nat_correct. cbn. all: eauto.
+      - repeat econstructor. now rewrite encode_nat_correct.
     }
   Qed.
 
 
-  (* More accurate termination time *)
-  (* This lemma demonstrates how to show termination of the [Match] operator, in case each case-machine has different/not constant run time. *)
-  Lemma MatchNat_Terminates :
-    projT1 MatchNat ↓
-           (fun tin k =>
-              exists m, tin[@Fin0] ≃ m /\
-                   match m with
-                   | O => 2 <= k
-                   | _ => 5 <= k
-                   end).
-  Proof.
-    eapply TerminatesIn_monotone.
-    { unfold MatchNat. repeat TM_Correct. }
-    {
-      intros tin i. intros (m&HEncM&Hi).
-      destruct HEncM as (y&ys&r1&HE1&HE2).
-      rewrite encode_nat_correct in HE1.
-      destruct m eqn:Em; cbn in *.
-      - exists 1, 0. repeat split.
-        + omega.
-        + omega.
-        + TMSimp. omega.
-      - exists 1, 3. repeat split.
-        + omega.
-        + omega.
-        + TMSimp. exists 1, 1. repeat split.
-          * omega.
-          * omega.
-          * TMSimp. omega.
-    }
-  Qed.
-
-  
-  (* Constructors *)
+  (** ** Constructors *)
   Section NatConstructor.
 
     Definition S_Rel : Rel (tapes (bool^+) 1) (unit * tapes (bool^+) 1) :=
       Mk_R_p (ignoreParam (fun tin tout => forall n : nat, tin ≃ n -> tout ≃ S n)).
 
     Definition Constr_S : { M : mTM (bool^+) 1 & states M -> unit } :=
-      Move _ L tt;; WriteMove (Some (inr true), L) tt;; WriteMove (Some (inl START), R) tt.
+      WriteMove (Some (inr true), L) tt;; Write (inl START) tt.
 
-    Lemma Constr_S_Sem : Constr_S ⊨c(5) S_Rel.
+
+    Lemma Constr_S_Sem : Constr_S ⊨c(3) S_Rel.
     Proof.
       eapply RealiseIn_monotone.
-      {
-        repeat eapply Seq_RealiseIn.
-        - eapply Move_Sem.
-        - eapply WriteMove_Sem.
-        - eapply WriteMove_Sem.
-      }
+      { unfold Constr_S. repeat TM_Correct. }
       { cbn. omega. }
       {
         intros tin (yout, tout) H. intros n HEncN.
-        TMSimp. clear H0 H4 H2 H3. simpl_tape.
-        destruct HEncN as (y&ys&r1&HE1&HE2).
-        rewrite encode_nat_correct in HE1.
-        destruct n as [ | n']; cbn in *; inv HE1.
-        - hnf. do 3 eexists. split.
-          + rewrite encode_nat_correct. cbn. reflexivity.
-          + cbn. f_equal. rewrite HE2. cbn. reflexivity.
-        - hnf. do 3 eexists. split.
-          + rewrite encode_nat_correct. cbn. reflexivity.
-          + cbn. f_equal. rewrite HE2. cbn. reflexivity.
+        TMSimp. clear all except HEncN. simpl_tape.
+        destruct HEncN as (r1&->). rewrite encode_nat_correct. cbn.
+        repeat econstructor. now rewrite encode_nat_correct.
       }
     Qed.
 
@@ -137,22 +81,19 @@ Section MatchNat.
 
 
     Definition Constr_O : { M : mTM (bool^+) 1 & states M -> unit } :=
-      WriteMove (Some (inr false), L) tt;;
-      WriteMove (Some (inl START), R) tt.
+        WriteMove (Some (inl STOP), L) tt;;
+        WriteMove (Some (inr false), L) tt;;
+        Write (inl START) tt.
 
-
-    Lemma Constr_O_Sem : Constr_O ⊨c(3) O_Rel.
+    Lemma Constr_O_Sem : Constr_O ⊨c(5) O_Rel.
     Proof.
       eapply RealiseIn_monotone.
       { unfold Constr_O. repeat TM_Correct. }
       { cbn. omega. }
       {
         intros tin (yout, tout) H.
-        intros HRight. TMSimp.
-        clear H H1 H2.
-        simpl_tape.
-        destruct HRight as (m&ls&HRight). rewrite HRight. cbn.
-        hnf. rewrite encode_nat_correct. cbn. repeat econstructor.
+        intros HRight. destruct HRight as (r1&r2&?). TMSimp. clear_all.
+        simpl_tape. repeat econstructor.
       }
     Qed.
 
